Add T_bot constructor to value types.

WebAssembly/Wasm.thy
@@ -147,8 +147,11 @@ inductive inst_typing :: "[s, inst, t_context] \<Rightarrow> bool" where
 inductive frame_typing :: "[s, f, t_context] \<Rightarrow> bool" where
 "\<lbrakk>list_all2 (\<lambda> v t. v_typing s v t) (f_locs f) tvs; inst_typing s (f_inst f) \<C>\<rbrakk> \<Longrightarrow> frame_typing s f (\<C>\<lparr>local := tvs\<rparr>)"
 
+(* n_zeros ts \<noteq> None precondition was added
+because t now contains not only value types
+but also T_bot. *)
 inductive cl_typing :: "[s, cl, tf] \<Rightarrow> bool" where
-   "\<lbrakk>inst_typing s i \<C>; tf = (t1s _> t2s); \<C>\<lparr>local := t1s @ ts, label := ([t2s] @ (label \<C>)), return := Some t2s\<rparr> \<turnstile> es : ([] _> t2s)\<rbrakk> \<Longrightarrow> cl_typing s (Func_native i tf ts es) (t1s _> t2s)"
+   "\<lbrakk>inst_typing s i \<C>; tf = (t1s _> t2s); \<C>\<lparr>local := t1s @ ts, label := ([t2s] @ (label \<C>)), return := Some t2s\<rparr> \<turnstile> es : ([] _> t2s); n_zeros ts \<noteq> None\<rbrakk> \<Longrightarrow> cl_typing s (Func_native i tf ts es) (t1s _> t2s)"
  |  "cl_typing s (Func_host tf h) tf"
 
 (* lifting the b_e_typing relation to the administrative operators *)
@@ -300,7 +303,7 @@ inductive reduce :: "[s, f, e list, s, f, e list] \<Rightarrow> bool" ("\<lparr>
 | call_indirect_Some:"\<lbrakk>(f_inst f) = i; stab s i ti (nat_of_int c) = Some (ConstRef i_cl); stypes i j = tf; cl_type (funcs s!i_cl) = tf\<rbrakk> \<Longrightarrow> \<lparr>s;f;[$EConstNum (ConstInt32 c), $(Call_indirect ti j)]\<rparr> \<leadsto> \<lparr>s;f;[Invoke i_cl]\<rparr>"
 | call_indirect_None:"\<lbrakk>(f_inst f) = i; (stab s i ti (nat_of_int c) = Some (ConstRef i_cl) \<and> stypes i j \<noteq> cl_type (funcs s!i_cl)) \<or> \<not> is_some_const_ref_func (stab s i ti (nat_of_int c))\<rbrakk> \<Longrightarrow> \<lparr>s;f;[$EConstNum (ConstInt32 c), $(Call_indirect ti j)]\<rparr> \<leadsto> \<lparr>s;f;[Trap]\<rparr>"
   \<comment> \<open>\<open>invoke\<close>\<close>
-| invoke_native:"\<lbrakk>(funcs s!i_cl) = Func_native j (t1s _> t2s) ts es; ves = ($C* vcs); length vcs = n; length ts = k; length t1s = n; length t2s = m; (n_zeros ts = zs) \<rbrakk> \<Longrightarrow> \<lparr>s;f;ves @ [Invoke i_cl]\<rparr> \<leadsto> \<lparr>s;f;[Frame m \<lparr> f_locs = vcs@zs, f_inst = j \<rparr> [(Label m [] ($*es))]]\<rparr>"
+| invoke_native:"\<lbrakk>(funcs s!i_cl) = Func_native j (t1s _> t2s) ts es; ves = ($C* vcs); length vcs = n; length ts = k; length t1s = n; length t2s = m; (n_zeros ts = Some zs) \<rbrakk> \<Longrightarrow> \<lparr>s;f;ves @ [Invoke i_cl]\<rparr> \<leadsto> \<lparr>s;f;[Frame m \<lparr> f_locs = vcs@zs, f_inst = j \<rparr> [(Label m [] ($*es))]]\<rparr>"
 | invoke_host_Some:"\<lbrakk>(funcs s!i_cl) = Func_host (t1s _> t2s) h; ves = ($C* vcs); length vcs = n; length t1s = n; length t2s = m; host_apply s (t1s _> t2s) h vcs hs (Some (s', vcs'))\<rbrakk> \<Longrightarrow> \<lparr>s;f;ves @ [Invoke i_cl]\<rparr> \<leadsto> \<lparr>s';f;($C* vcs')\<rparr>"
 | invoke_host_None:"\<lbrakk>(funcs s!i_cl) = Func_host (t1s _> t2s) h; ves = ($C* vcs); length vcs = n; length t1s = n; length t2s = m\<rbrakk> \<Longrightarrow> \<lparr>s;f;ves @ [Invoke i_cl]\<rparr> \<leadsto> \<lparr>s;f;[Trap]\<rparr>"
   \<comment> \<open>\<open>references\<close>\<close>
